cleaned it up

Caches/StoreAtomicity.v
@@ -2,7 +2,26 @@ Require Import DataTypes Transitions.
 
 Set Implicit Arguments.
 
-Section StoreAtomicity.
+Inductive InstantMemory : (Addr -> Data) -> (Addr -> Data) -> Set :=
+| IReq m a (p: Proc) d (w: Desc):
+  InstantMemory m (if w
+                   then m
+                   else 
+                     fun a' => 
+                       if decAddr a a'
+                       then d
+                       else m a')
+| IIdle m: InstantMemory m m.
+
+Definition getImIo s s' (t: InstantMemory s s') :=
+  match t with
+    | IReq m a p d w => Some (a, p, d, w, if w
+                                          then m a
+                                          else initData zero)
+    | IIdle m => None
+  end.
+
+Section CreateInstantMemory.
   Variable State: Set.
   Variable Trans: AllTransitions State.
   Variable initState: State.
@@ -11,7 +30,7 @@ Section StoreAtomicity.
 
   Record StoreAtomicity := {
    storeAtomicityLd:
-    forall a c d ld t,
+    forall t a c d ld,
       getStreamIo getTransIo t stm = Some (a, c, d, Ld, ld) ->
       (d = initData zero /\ ld = initData a /\
      forall {ti}, 0 <= ti < t -> forall ci di ldi, defined ci ->
@@ -22,7 +41,44 @@ Section StoreAtomicity.
                      ~ getStreamIo getTransIo ti stm = Some (a, ci, di, St, ldi));
 
    storeAtomicitySt:
-   forall a c d ld t,
+   forall t a c d ld,
      getStreamIo getTransIo t stm = Some (a, c, d, St, ld) ->
      ld = initData zero}.
-End StoreAtomicity.
+
+  CoFixpoint buildIm n m: Stream InstantMemory m :=
+  TCons _ (match getStreamIo getTransIo n stm as use
+              return (InstantMemory m match use with
+                                        | Some (a, _, d, w, _) => if w
+                                                                  then m
+                                                                  else fun a' =>
+                                                                         if decAddr a a'
+                                                                         then d
+                                                                         else m a'
+                                        | None => m
+                                      end) with
+             | Some (a, c, d, w, ld) => (IReq m a c d w)
+             | None => (IIdle m)
+           end) (buildIm (S n) (match getStreamIo getTransIo n stm as use
+                                   return (Addr -> Data) with
+                                  | Some (a, c, d, w, ld) => if w
+                                                             then m
+                                                             else fun a' =>
+                                                                    if decAddr a a'
+                                                                    then d
+                                                                    else m a'
+                                  | None => m
+                                end)).
+End CreateInstantMemory.
+
+Section AllSa.
+  Variable stm: Stream InstantMemory initData.
+
+(*
+  Theorem stmSa: StoreAtomicity stm getImIo.
+  Proof.
+    constructor.
+
+    induction t.
+    intros.
+*)
+End AllSa.
